server invs

src/program_proof/pav/invs.v
@@ -5,8 +5,16 @@ From iris.unstable.base_logic Require Import mono_list.
 From Perennial.base_logic.lib Require Import ghost_map.
 From Perennial.algebra Require Import ghost_map_pers.
 
+Section shared.
+Class pavG Σ :=
+  {
+    mono_trees :> mono_listG gname Σ;
+    tree_maps :> ghost_mapG Σ (list w8) (list w8);
+  }.
+End shared.
+
 Section epochChain.
-Context `{!heapGS Σ}.
+Context `{!heapGS Σ, !pavG Σ}.
 
 Definition chainSepNone_hashes_to h : iProp Σ :=
   is_hash [(W8 0)] h.
@@ -31,7 +39,7 @@ Proof. Admitted.
 End epochChain.
 
 Section global_inv.
-Context `{!heapGS Σ, !mono_listG gname Σ, !ghost_mapG Σ (list w8) (list w8)}.
+Context `{!heapGS Σ, !pavG Σ}.
 (* state is tied together as follows, all from one γ:
 γ →[mono_list]
 γtrees →[ghost_map_auth]
@@ -48,7 +56,7 @@ Definition global_inv γ : iProp Σ :=
 End global_inv.
 
 Section serv_sigpreds.
-Context `{!heapGS Σ, !mono_listG gname Σ, !ghost_mapG Σ (list w8) (list w8)}.
+Context `{!heapGS Σ, !pavG Σ}.
 
 Definition serv_sigpred_link γ (data : servSepLink.t) : iProp Σ :=
   ∃ (epoch : w64) (prevLink dig : list w8) γtrees trees digs links,
